\documentclass[12pt]{article}
\usepackage{latexsym}
\usepackage{lipsum}
\usepackage{graphicx}
\usepackage{float}
\usepackage{mathtools}
\usepackage{framed}
\usepackage[margin=1in]{geometry} 
\usepackage{amsmath,amsthm,amssymb}
\usepackage{caption}

\setlength\parindent{24pt}
\textwidth     =  6.5in
\textheight    =  8.2in
\oddsidemargin =  -0.2in
\topmargin     = -0.4in
%%%%%%%%%%%%%%%%%%%%%%%%%%%%%%%%%%%%%%%%%%%%%%%%%%%%%%%%%%%%%%%%%%%%%%%%

\newcommand{\real}{\mathbb{R}}
\newcommand{\complex}{\mathbb{C}}
\newcommand{\feal}{\mathbb{F}}
\newcommand{\ul}{\underline}

%\input{header}
%
\newcommand{\noi}{\noindent}
\newcommand{\pa}{\partial}
%
\newcommand{\bea}{\begin{eqnarray}}
\newcommand{\eea}{\end{eqnarray}}
%
\newcommand{\beas}{\begin{eqnarray*}}
\newcommand{\eeas}{\end{eqnarray*}}
%
\newcommand{\non}{\nonumber}
%
\newcommand{\bit}{\begin{itemize}}
\newcommand{\eit}{\end{itemize}}
%
\newcommand{\bee}{\begin{enumerate}}
\newcommand{\eee}{\end{enumerate}}
%
\newcommand{\bed}{\begin{description}}
\newcommand{\edd}{\end{description}}
%
\newcommand{\bec}{\begin{center}}
\newcommand{\edc}{\end{center}}
%
\renewcommand{\thefootnote}{\roman{footnote}}
%
%%%%%%%%%%%%%%%%%%%%%%%%%%%%%%%%%%%%%%%
%%%%%%%%%%%%%%%%%%%%%%%%%%%%%%%%%%%%%%%
%%%%%%%%%%%%%%%%%%%%%%%%%%%%%%%%%%%%%%%
\begin{document}

\[
\frac{-x}{1-x}-\ln(1-x)=h\left(\frac{1}{1-x}\right)\leq 0
\]
\[
\ln(1-\bar{c}\epsilon_k) \geq \frac{-\bar{c}\epsilon_k}{1-\bar{c}\epsilon_k} \geq -2\bar{c}\epsilon_k
\]
\bea \label{6.59}
\ln( \tilde{m_k} )\geq \ln(1-\bar{c}\epsilon_k) \geq -2\bar{c}\epsilon_k \geq -2c\epsilon_k
\eea
\bea \label{6.60}
0<\psi(\tilde{B_{k+1}}) \leq \psi(\tilde{B_{k}}) + 3c\epsilon_k + \ln(cos^2\tilde{\theta_k} )+ \left[ 1- \frac{\tilde{q_k}}{cos^2\tilde{\theta_k}} + \ln\left(\frac{\tilde{q_k}}{cos^2\tilde{\theta_k}}\right) \right]
\eea
\[
\sum\limits_{j=0}^\infty \left(\ln\left(\frac{1}{cos^2\tilde{\theta_j}}\right) - \left[ 1- \frac{\tilde{q_j}}{cos^2\tilde{\theta_j}} + \ln\left(\frac{\tilde{q_j}}{cos^2\tilde{\theta_j}}\right) \right]\right) \leq \psi(\tilde{B_0})+3c\sum\limits_{j=0}^\infty \epsilon_j < +\infty
\]
\[
\lim_{j\to\infty} \ln\left( \frac{1}{cos^2\tilde{\theta_j}}\right)=0, \ \ \ \ \ \ \ \ \ \ \ \ \ \ \ 
\lim_{j\to\infty} \left( 1- \frac{\tilde{q_j}}{cos^2\tilde{\theta_j}} + \ln\left(\frac{\tilde{q_j}}{cos^2\tilde{\theta_j}} \right)\right) = 0
\]
\bea \label{6.61}
\lim_{j\to\infty} cos\tilde{\theta_j}=1,  \ \ \ \ \ \ \ \ 
\lim_{j\to\infty} \tilde{q_j}=1
\eea



 
\end{document}